theories/Weakening.v
@@ -3,36 +3,67 @@ From LogRel.AutoSubst Require Import core unscoped Ast.
 From LogRel Require Import Utils BasicAst Notations Context Untyped.
 
 Inductive weakening : Set :=
-  | wk_id : weakening
-  | wk_step (w : weakening) : weakening
-  | wk_up (w : weakening) : weakening.
+  | _wk_empty : weakening
+  | _wk_step (w : weakening) : weakening
+  | _wk_up (w : weakening) : weakening.
+
+Fixpoint _wk_id (Γ : context) : weakening :=
+  match Γ with
+    | nil => _wk_empty
+    | cons _ Γ' => _wk_up (_wk_id Γ')
+  end.
 
 (* Transforms an (intentional) weakening into a renaming *)
 Fixpoint wk_to_ren (ρ : weakening) : nat -> nat :=
   match ρ with
-    | wk_id => id
-    | wk_step ρ' => (wk_to_ren ρ') >> S
-    | wk_up ρ' => up_ren (wk_to_ren ρ')
+    | _wk_empty => id
+    | _wk_step ρ' => (wk_to_ren ρ') >> S
+    | _wk_up ρ' => up_ren (wk_to_ren ρ')
   end.
+
+Lemma wk_to_ren_id Γ : (wk_to_ren (_wk_id Γ)) =1 id.
+Proof.
+  induction Γ.
+  1: reflexivity.
+  intros [] ; cbn.
+  2: rewrite IHΓ.
+  all: reflexivity.
+Qed.
+
 Coercion wk_to_ren : weakening >-> Funclass.
 
 #[global] Instance RenWk_term : (Ren1 weakening term term) :=
   fun ρ t => ren_term (wk_to_ren ρ) t.
 
+Arguments RenWk_term /.
+
 Inductive well_weakening : weakening -> context -> context -> Type :=
-  | well_id (Γ : context) : well_weakening wk_id Γ Γ
-  | well_step (Γ Δ : context) (na : aname) (A : term) (ρ : weakening) :
-    well_weakening ρ Γ Δ -> well_weakening (wk_step ρ) (Γ,,vass na A) Δ
-  | well_up (Γ Δ : context) (na : aname) (A : term) (ρ : weakening) :
-    well_weakening ρ Γ Δ -> well_weakening (wk_up ρ) (Γ,,vass na A⟨ρ⟩) (Δ,, vass na A).
+  | well_empty : well_weakening _wk_empty ε ε
+  | well_step {Γ Δ : context} (na : aname) (A : term) (ρ : weakening) :
+    well_weakening ρ Γ Δ -> well_weakening (_wk_step ρ) (Γ,,vass na A) Δ
+  | well_up {Γ Δ : context} (na : aname) (A : term) (ρ : weakening) :
+    well_weakening ρ Γ Δ -> well_weakening (_wk_up ρ) (Γ,,vass na (ren_term ρ A)) (Δ,, vass na A).
+
+Lemma well_wk_id (Γ : context) : well_weakening (_wk_id Γ) Γ Γ.
+Proof.
+  induction Γ as [|d].
+  1: econstructor.
+  replace d with (d⟨wk_to_ren (_wk_id Γ)⟩) at 2.
+  all: destruct d as [na A].
+  1: now econstructor.
+  cbn.
+  f_equal.
+  rewrite wk_to_ren_id.
+  now asimpl.
+Qed.
 
 Fixpoint wk_compose (ρ ρ' : weakening) : weakening :=
   match ρ, ρ' with
-    | wk_id, _ => ρ'
-    | wk_step ν , _ => wk_step (wk_compose ν ρ')
-    | wk_up ν, wk_id => ρ
-    | wk_up ν, wk_step ν' => wk_step (wk_compose ν ν')
-    | wk_up ν, wk_up ν' => wk_up (wk_compose ν ν')
+    | _wk_empty , _ => ρ'
+    | _wk_step ν , _ => _wk_step (wk_compose ν ρ')
+    | _wk_up ν, _wk_empty => ρ
+    | _wk_up ν, _wk_step ν' => _wk_step (wk_compose ν ν')
+    | _wk_up ν, _wk_up ν' => _wk_up (wk_compose ν ν')
   end.
 
 Lemma wk_compose_compose (ρ ρ' : weakening) : wk_to_ren (wk_compose ρ ρ') =1 ρ' >> ρ.
@@ -62,7 +93,7 @@ Proof.
   - eassumption.
   - econstructor. auto.
   - inversion H' as [| | ? ? na' A' ν']; subst ; clear H'.
-    1-2: now econstructor ; auto.
+    1: now econstructor ; auto.
     asimpl.
     replace (ren_term (ν' >> ν) A') with (ren_term (wk_compose ν ν') A')
       by now rewrite wk_compose_compose.
@@ -75,10 +106,23 @@ Arguments wk_well_wk : clear implicits.
 Arguments Build_wk_well_wk : clear implicits.
 Notation "Γ ≤ Δ" := (wk_well_wk Γ Δ).
 
+Definition wk_empty : (ε ≤ ε) := {| wk := _wk_empty ; well_wk := well_empty |}.
+
+Definition wk_step {Γ Δ} na A (ρ : Γ ≤ Δ) : (Γ,, vass na A) ≤ Δ :=
+  {| wk := _wk_step ρ ; well_wk := well_step na A ρ ρ |}.
+
+Definition wk_up {Γ Δ} na A (ρ : Γ ≤ Δ) : (Γ,, vass na A⟨wk_to_ren ρ⟩) ≤ (Δ ,, vass na A) :=
+  {| wk := _wk_up ρ ; well_wk := well_up na A ρ ρ |}.
+
+Definition wk_id {Γ} : Γ ≤ Γ :=
+  {| wk := _wk_id Γ ; well_wk := well_wk_id Γ |}.
+
 #[global] Hint Resolve well_wk : core.
 
 #[global] Instance RenWlWk_term {Γ Δ : context }: (Ren1 (Γ ≤ Δ) term term) :=
   fun ρ t => ren_term (wk_to_ren ρ.(wk)) t.
+
+Arguments RenWlWk_term /.
 
 Definition wk_well_wk_compose {Γ Γ' Γ'' : context} (ρ : Γ ≤ Γ') (ρ' : Γ' ≤ Γ'') : Γ ≤ Γ'' :=
   {| wk := wk_compose ρ.(wk) ρ'.(wk) ; well_wk := well_wk_compose ρ.(well_wk) ρ'.(well_wk) |}.
@@ -92,7 +136,7 @@ Proof.
 Qed.
 
 (* Testing that the definitions are right *)
-Lemma id_ren (Γ : context) (ρ : Γ ≤ Γ) : (wk_to_ren ρ) =1 id.
+Lemma id_ren (Γ : context) (ρ : Γ ≤ Γ) : ρ =1 id.
 Proof.
   destruct ρ as [ρ wellρ].
   cbn in *.
@@ -142,10 +186,46 @@ Proof.
   - destruct n ; cbn.
     + cbn.
       inversion Hdecl ; subst ; clear Hdecl.
-      unfold ren1, Ren_decl.
+      cbn -[map_decl].
       rewrite map_decl_lift.
       now constructor.
     + inversion Hdecl ; subst ; cbn in *.
       rewrite map_decl_lift.
       now econstructor.
   Qed.
+
+Section RenWhnf.
+
+  Variable (ρ : nat -> nat).
+
+  Lemma whne_ren t : whne t -> whne (ren_term ρ t).
+  Proof.
+    induction 1 ; cbn.
+    all: now econstructor.
+  Qed.
+
+  Lemma whnf_ren t : whnf t -> whnf (ren_term ρ t).
+  Proof.
+    induction 1 ; cbn.
+    all: econstructor.
+    now eapply whne_ren.
+  Qed.
+  
+  Lemma isType_ren A : isType A -> isType (ren_term ρ A).
+  Proof.
+    induction 1 ; cbn.
+    all: econstructor.
+    now eapply whne_ren.
+  Qed.
+  
+  Lemma isFun_ren f : isFun f -> isFun (ren_term ρ f).
+  Proof.
+    induction 1 ; cbn.
+    all: econstructor.
+    now eapply whne_ren.
+  Qed.
+
+End RenWhnf.
+
+#[global] Hint Resolve whne_ren whnf_ren isType_ren isFun_ren : gen_typing.
+
