theories/AlgorithmicTypingProperties.v
@@ -1,0 +1,638 @@
+From LogRel.AutoSubst Require Import core unscoped Ast.
+From LogRel Require Import Utils BasicAst Notations Context Untyped Weakening UntypedReduction
+  GenericTyping DeclarativeTyping Generation Reduction AlgorithmicTyping.
+
+Import AlgorithmicTypingData DeclarativeTypingProperties.
+
+Lemma infer_red_equiv Γ t A :
+  InferRedAlg Γ A t <~> [Γ |-[al] t ▹h A].
+Proof.
+  split ; intros [] ; now econstructor.
+Qed.
+
+Section AlgTypingWh.
+
+  Let PTy (Γ : context) (A : term) := True.
+  Let PInf (Γ : context) (A t : term) := True.
+  Let PInfRed (Γ : context) (A t : term) := True.
+  Let PCheck (Γ : context) (A t : term) := True.
+  Let PTyEq (Γ : context) (A B : term) := True.
+  Let PTyRedEq (Γ : context) (A B : term) := 
+    isType A × isType B.
+  Let PNeEq (Γ : context) (A t u : term) := 
+    whne t × whne u.
+  Let PNeRedEq (Γ : context) (A t u : term) :=
+    whne t × whne u.
+  Let PTmEq (Γ : context) (A t u : term) := True.
+  Let PTmRedEq (Γ : context) (A t u : term) := 
+    [× whnf t, whnf u & isType A].
+
+  Theorem typing_alg_wh :
+    WfAlgoInductionConcl PTy PInf PInfRed PCheck PTyEq PTyRedEq
+      PNeEq PNeRedEq PTmEq PTmRedEq.
+  Proof.
+    subst PTy PInf PInfRed PCheck PTyEq PTyRedEq
+      PNeEq PNeRedEq PTmEq PTmRedEq.
+    apply WfAlgoInduction.
+    all: try solve [now constructor].
+    all: intros ;
+      repeat match goal with
+      | H : [× _, _ & _] |- _ => destruct H
+      | H : _ × _ |- _ => destruct H
+      end.
+    all: try solve [now do 2 constructor].
+    constructor.
+    1-2: gen_typing.
+    now constructor.
+  Qed.
+End AlgTypingWh.
+
+Conjecture typing_subst : WfDeclInductionConcl
+  (fun _ => True)
+  (fun Γ A => forall Δ σ, [|-[de] Δ] -> [Δ |-[de]s σ : Γ] -> [Δ |-[de] A[σ]])
+  (fun Γ A t => forall Δ σ, [|-[de] Δ] -> [Δ |-[de]s σ : Γ] -> [Δ |-[de] t[σ] : A[σ]])
+  (fun Γ A B => forall Δ σ σ', [|-[de] Δ] -> [Δ |-[de]s σ ≅ σ' : Γ] -> [Δ |-[de] A[σ] ≅ B[σ']])
+  (fun Γ A t u => forall Δ σ σ', [|-[de] Δ] -> [Δ |-[de]s σ ≅ σ' : Γ] -> [Δ |-[de] t[σ] ≅ u[σ'] : A[σ]]).
+
+Conjecture validity : WfDeclInductionConcl
+  (fun _ => True)
+  (fun _ _ => True)
+  (fun Γ A t => [Γ |-[de] A])
+  (fun Γ A B => [Γ |-[de] A] × [Γ |-[de] B])
+  (fun Γ A t u => [× [Γ |-[de] A], [Γ |-[de] t : A] & [Γ |- u : A]]).
+
+Conjecture prod_ty_inj : forall Γ na A B na' A' B',
+  [Γ |-[de] tProd na A B ≅ tProd na' A' B'] ->
+  [Γ |-[de] A' ≅ A] × [Γ,, vass na A |-[de] B ≅ B'].
+
+Conjecture prod_tm_inj : forall Γ na A B na' A' B',
+  [Γ |-[de] tProd na A B ≅ tProd na' A' B' : U ] ->
+  [Γ |-[de] A' ≅ A : U ] × [Γ,, vass na A |-[de] B ≅ B' : U].
+
+Conjecture app_neu_inj : forall Γ m t n u T,
+  whne m ->
+  whne n ->
+  [Γ |-[de] tApp m t ≅ tApp n u : T] ->
+  ∑ na A B, [×
+    [Γ |-[de] m ≅ n : tProd na A B],
+    [Γ |-[de] t ≅ u : A] &
+    [Γ |-[de] B[t..] ≅ T]].
+
+Conjecture prod_ty_red_compl : forall Γ na A B T,
+  [Γ |-[de] tProd na A B ≅ T] ->
+  ∑ na' A' B', [Γ |-[de] T ⇒* tProd na' A' B'].
+
+Conjecture prod_tm_red_compl : forall Γ na A B T,
+  [Γ |-[de] tProd na A B ≅ T : U] ->
+  ∑ na' A' B', [Γ |-[de] T ⇒* tProd na' A' B' : U].
+
+Conjecture univ_red_compl : forall Γ T,
+  [Γ |-[de] U ≅ T] ->
+  [Γ |-[de] T ⇒* U].
+
+Section Stability.
+
+  Lemma ctx_conv_refl Γ :
+    [|-[de] Γ] ->
+    [|-[de] Γ ≅ Γ].
+  Proof.
+    induction 1.
+    all: constructor ; tea.
+    now eapply TypeRefl.
+  Qed.
+
+  Lemma wk_subst_compose (Γ Δ Δ' : context) (ρ : Δ' ≤ Δ) σ :
+    [|- Δ'] ->
+    [Δ |-s σ : Γ] ->
+    [Δ' |-s σ >> ⟨ρ⟩ : Γ].
+  Proof.
+    intros ?.
+    induction 1 as [|σ Γ na A].
+    1: now econstructor.
+    econstructor.
+    - asimpl ; cbn in * ; asimpl.
+      eassumption.
+    - asimpl ; cbn in * ; asimpl.
+      unfold funcomp.
+      eapply typing_meta_conv.
+      1: eapply typing_wk ; eassumption.
+      asimpl.
+      reflexivity.
+  Qed.
+
+  Lemma well_subst_up (Γ Δ : context) na A σ :
+    [Δ |- A] ->
+    [Δ |-s σ : Γ] ->
+    [Δ ,, vass na A |-s σ >> ⟨↑⟩ : Γ].
+  Proof.
+    intros HA Hσ.
+    unshelve eapply (wk_subst_compose _ _ (Δ,, vass na A)) in Hσ.
+    - now eapply wk_step, wk_id.
+    - eapply well_subst_ext ; [|eassumption].
+      asimpl ; cbn in * ; asimpl.
+      rewrite wk_to_ren_id.
+      now reflexivity.
+    - econstructor ; fold_decl.
+      all: gen_typing.
+  Qed.
+
+  Lemma id_subst (Γ : context) :
+    [|- Γ] ->
+    [Γ |-s tRel : Γ].
+  Proof.
+    induction 1.
+    all: econstructor.
+    - eapply well_subst_ext.
+      2: now eapply well_subst_up.
+      now asimpl.
+    - eapply typing_meta_conv.
+      1: now do 2 econstructor.
+      cbn ; now renamify.
+  Qed.
+
+  Lemma wf_subst (Γ Δ : context) :
+    [ |- Γ ≅ Δ] ->
+    [|- Γ].
+  Proof.
+    destruct 1 as [| ? ? ? ? ? ? ? HA].
+    all: econstructor ; fold_decl.
+    - gen_typing.
+    - now eapply validity in HA.
+  Qed.
+
+  Lemma subst_refl (Γ Δ : context) σ :
+    [Γ |-[de]s σ : Δ] ->
+    [Γ |-[de]s σ ≅ σ : Δ].
+  Proof.
+    induction 1.
+    all: econstructor ; tea.
+    now eapply TermRefl.
+  Qed.
+
+  Lemma conv_well_subst (Γ Δ : context) :
+    [ |- Γ ≅ Δ] ->
+    [Γ |-[de]s tRel : Δ].
+  Proof.
+    induction 1 as [| * ? HA].
+    - now econstructor.
+    - assert [Γ |-[de] A] by
+        now eapply validity in HA as [].
+      assert [|-[de] Γ,, vass na A] by
+        (econstructor ; fold_decl ;
+        eauto using wf_subst).
+      econstructor ; fold_decl ; tea.
+      + eapply well_subst_ext, well_subst_up ; tea.
+        reflexivity.
+      + econstructor.
+        1: now econstructor ; [..|econstructor].
+        cbn ; renamify.
+        unshelve eapply typing_wk in HA.
+        2: eapply wk_step, wk_id.
+        2: eassumption.
+        unshelve erewrite (extRen_term _ _ _ B), (extRen_term _ _ _ A).
+        5: eassumption.
+        all: now intros ; cbn ; rewrite wk_to_ren_id.
+  Qed.
+
+  Let PCon (Γ : context) := True.
+  Let PTy (Γ : context) (A : term) := forall Δ,
+    [|-[de] Δ ≅ Γ] -> [Δ |- A].
+  Let PTm (Γ : context) (A t : term) := forall Δ,
+    [|-[de] Δ ≅ Γ] -> [Δ |- t : A].
+  Let PTyEq (Γ : context) (A B : term) := forall Δ,
+    [|-[de] Δ ≅ Γ] -> [Δ |- A ≅ B].
+  Let PTmEq (Γ : context) (A t u : term) := forall Δ,
+    [|-[de] Δ ≅ Γ] -> [Δ |- t ≅ u : A].
+
+  Theorem stability : WfDeclInductionConcl PCon PTy PTm PTyEq PTmEq.
+  Proof.
+    red.
+    repeat match goal with |- _ × _ => split end.
+    1: now unfold PCon.
+    all: intros * Hty Δ HΔ.
+    all: pose proof (wf_subst _ _ HΔ).
+    all: eapply conv_well_subst in HΔ.
+    all: pose proof (subst_refl _ _ _ HΔ).
+    all: eapply typing_subst in Hty ; tea.
+    all: repeat (rewrite idSubst_term in Hty ; [..|reflexivity]).
+    all: try eassumption.
+  Qed.
+
+End Stability.
+
+Section Soundness.
+
+  Lemma termGen' Γ t A :
+    [Γ |- t : A] ->
+    ∑ A', (termGenData Γ t A') × [Γ |- A' ≅ A].
+  Proof.
+    intros * H.
+    destruct (termGen _ _ _ H) as [? [? [->|]]].
+    2: now eexists.
+    eexists ; split ; tea.
+    eapply TypeRefl.
+    now eapply validity in H.
+  Qed.
+
+  Theorem subject_reduction_one Γ t t' A :
+    [Γ |-[de] t : A] ->
+    [t ⇒ t'] ->
+    [Γ |- t ⇒ t' : A].
+  Proof.
+    intros Hty Hred.
+    induction Hred in Hty, A |- *.
+    - apply termGen' in Hty as [? [Hty Heq]].
+      inversion Hty; subst ; clear Hty.
+      apply termGen' in H1 as [? [Hty Heq']].
+      inversion Hty ; subst ; clear Hty.
+      eapply prod_ty_inj in Heq' as [? HeqB].
+      econstructor ; fold_decl.
+      1: econstructor ; fold_decl ; gen_typing.
+      etransitivity ; tea.
+      eapply typing_subst ; tea.
+      1: now gen_typing.
+      econstructor ; cbn.
+      all: asimpl.
+      2: eapply TermRefl ; fold_decl ; gen_typing.
+      now eapply subst_refl, id_subst ; gen_typing.
+    - apply termGen' in Hty as [? [Hty Heq]].
+      inversion Hty ; subst ; clear Hty.
+      econstructor ; tea.
+      econstructor.
+      1: easy.
+      fold_decl ; gen_typing.
+    Qed.
+
+  Theorem subject_reduction Γ t t' A :
+    [Γ |-[de] t : A] ->
+    [t ⇒* t'] ->
+    [Γ |- t ⇒* t' : A].
+  Proof.
+    intros Hty.
+    induction 1 as [| ? ? ? o red] in A, Hty |- *.
+    1: now econstructor.
+    eapply subject_reduction_one in o ; tea.
+    etransitivity.
+    2: eapply IHred.
+    1: now constructor.
+    now eapply RedConvTe, validity in o as [].
+  Qed.
+
+  Lemma subject_reduction_one_type Γ A A' :
+    [Γ |- A] ->
+    [A ⇒ A'] ->
+    [Γ |- A ⇒ A'].
+  Proof.
+    intros Hty.
+    inversion 1 ; subst.
+    all: inversion Hty ; subst ; clear Hty.
+    all: econstructor.
+    all: now eapply subject_reduction_one.
+  Qed.
+
+  Theorem subject_reduction_type Γ A A' :
+  [Γ |- A] ->
+  [A ⇒* A'] ->
+  [Γ |- A ⇒* A'].
+  Proof.
+    intros Hty.
+    induction 1 as [| ? ? ? o red] in Hty |- *.
+    1: now econstructor.
+    eapply subject_reduction_one_type in o ; tea.
+    etransitivity.
+    2: eapply IHred.
+    1: now constructor.
+    now eapply RedConvTy, validity in o as [].
+  Qed.
+
+  Lemma typing_eta' (Γ : context) na A B f :
+    [Γ |- f : tProd na A B] ->
+    [Γ,, vass na A |- eta_expand f : B].
+  Proof.
+    intros Hf.
+    eapply typing_eta ; tea.
+    - gen_typing.
+    - eapply validity in Hf.
+      inversion Hf ; subst ; tea.
+      eapply termGen' in H as [? [H ?]]; inversion H ; subst ; clear H.
+      now econstructor.
+    - eapply validity in Hf.
+      inversion Hf ; subst ; tea.
+      eapply termGen' in H as [? [H ?]]; inversion H ; subst ; clear H.
+      now econstructor.
+  Qed.
+
+  Let PTy (Γ : context) (A : term) :=
+    [|-[de] Γ] -> [Γ |-[de] A].
+  Let PInf (Γ : context) (A t : term) :=
+    [|-[de] Γ] ->
+    [Γ |-[de] t : A].
+  Let PCheck (Γ : context) (A t : term) :=
+    [Γ |-[de] A] ->
+    [Γ |-[de] t : A].
+  Let PTyEq (Γ : context) (A B : term) :=
+    [Γ |-[de] A] ->
+    [Γ |-[de] B] ->
+    [Γ |-[de] A ≅ B].
+  Let PTmEq (Γ : context) (A t u : term) :=
+    [Γ |-[de] t : A] -> [Γ |-[de] u : A] ->
+    [Γ |-[de] t ≅ u : A].
+  Let PNeEq (Γ : context) (A : term) (m n : term) :=
+    (∑ T, [Γ |-[de] m : T]) ->
+    (∑ T, [Γ |-[de] n : T]) ->
+    [× [Γ |-[de] m ≅ n : A],
+      (forall T, [Γ |-[de] m : T] -> [Γ |-[de] A ≅ T]) &
+      (forall T, [Γ |-[de] n : T] -> [Γ |-[de] A ≅ T])].
+
+  Theorem typing_sound :
+    WfAlgoInductionConcl PTy PInf PInf PCheck PTyEq PTyEq
+      PNeEq PNeEq PTmEq PTmEq.
+  Proof.
+    subst PTy PInf PCheck PTyEq PNeEq PTmEq.
+    apply WfAlgoInduction.
+    - now econstructor.
+    - econstructor ; fold_decl ; gen_typing.
+    - econstructor ; fold_decl ; gen_typing.
+    - econstructor ; fold_decl ; gen_typing.
+    - econstructor ; fold_decl ; gen_typing.
+    - econstructor ; fold_decl ; gen_typing.
+    - intros * ? IHf ? IHA.
+      econstructor ; fold_decl.
+      1: gen_typing.
+      eapply validity, prod_ty_inv in IHf as [] ; tea.
+      now gen_typing.
+    - intros * ? IHt HA ?.
+      eapply subject_reduction_type, RedConvTyC in HA.
+      2: now eapply validity in IHt.
+      gen_typing.
+    - intros * ? IHt ? IHA ?.
+      unshelve epose proof (IHA _ _) ; tea.
+      1: eapply validity in IHt.
+      all: gen_typing.
+    - intros * HA HB ? IHA' ? ?.
+      eapply subject_reduction_type, RedConvTyC in HA, HB ; tea.
+      unshelve epose proof (IHA' _ _).
+      1-2: now eapply validity in HA, HB.
+      symmetry in HB.
+      do 2 etransitivity ; tea.
+      now eapply TypeRefl.
+    - intros * ? IHA ? IHB ? ?.
+      eapply prod_ty_inv in H1 as [], H2 as [].
+      econstructor ; fold_decl ; tea.
+      1: now eauto.
+      eapply IHB.
+      1: eauto.
+      eapply stability ; tea.
+      econstructor.
+      2: now eauto.
+      eapply ctx_conv_refl.
+      now gen_typing.
+    - now gen_typing.
+    - intros * Hconv IH HM HN.
+      eapply typing_alg_wh in Hconv as [neM neN].
+      eapply convUniv ; fold_decl.
+      inversion HM ; subst ; clear HM.
+      1-2: now inversion neM.
+      inversion HN ; subst ; clear HN.
+      1-2: now inversion neN.
+      now eapply IH.
+    - intros * Hin []  _.
+      split.
+      + do 2 constructor ; fold_decl ; gen_typing.
+      + intros T Hty.
+        eapply termGen' in Hty as [? [Hty ?]].
+        inversion Hty ; subst ; clear Hty.
+        eapply in_ctx_inj in Hin ; tea ; subst.
+        eassumption.
+      + intros T Hty.
+        eapply termGen' in Hty as [? [Hty ?]].
+        inversion Hty ; subst ; clear Hty.
+        eapply in_ctx_inj in Hin ; tea ; subst.
+        eassumption.
+    - intros * ? IHm ? IHt [? Htym] [? Htyn].
+      eapply termGen' in Htym as [? [Htym ?]].
+      inversion Htym ; subst ; clear Htym.
+      eapply termGen' in Htyn as [? [Htyn ?]].
+      inversion Htyn ; subst ; clear Htyn.
+      edestruct IHm as [IHmc IHm' IHn'].
+      1-2: now econstructor.
+      eapply IHm', prod_ty_inj in H3 as [].
+      eapply IHn', prod_ty_inj in H4 as [].
+      split.
+      + econstructor ; fold_decl ; gen_typing.
+      + intros ? Happ.
+        eapply termGen' in Happ as [? [Happ ?]].
+        inversion Happ ; subst ; clear Happ.
+        eapply IHm', prod_ty_inj in H3 as [].
+        etransitivity ; [..|eassumption].
+        eapply typing_subst.
+        1-2: gen_typing.
+        econstructor ; asimpl.
+        1: eapply subst_refl, id_subst.
+        2: eapply TermRefl ; fold_decl.
+        all: now gen_typing.
+      + intros ? Happ.
+        eapply termGen' in Happ as [? [Happ ?]].
+        inversion Happ ; subst ; clear Happ.
+        eapply IHn', prod_ty_inj in H3 as [].
+        etransitivity ; [..|eassumption].
+        eapply typing_subst.
+        1-2: gen_typing.
+        econstructor ; asimpl.
+        1: eapply subst_refl, id_subst.
+        all: now gen_typing.
+    - intros * ? IHm HA [? Htym] [? Htyn].
+      edestruct IHm as [IHmc IHm' IHn'].
+      1-2: now eexists.
+      eapply subject_reduction_type, RedConvTyC in HA.
+      2: now eapply validity in IHmc as [].
+      split.
+      + gen_typing.
+      + intros.
+        symmetry in HA.
+        etransitivity ; gen_typing.
+      + intros.
+        symmetry in HA.
+        etransitivity ; gen_typing.
+    - intros * HA Ht Hu ? IH Htyt Htyu.
+      eapply subject_reduction_type, RedConvTyC in HA.
+      2: now eapply validity in Htyt.
+      eapply subject_reduction, RedConvTeC in Ht ; tea.
+      eapply subject_reduction, RedConvTeC in Hu ; tea.
+      etransitivity ; [..|etransitivity].
+      1: eassumption.
+      2: now symmetry.
+      eapply TermConv ; fold_decl.
+      2: now symmetry.
+      eapply IH.
+      all: econstructor ; fold_decl ; tea.
+      all: now eapply validity in Ht as [], Hu as [].
+    - intros * ? IHA ? IHB Hty Hty'.
+      eapply termGen' in Hty as [? [Hty _]].
+      inversion Hty ; subst ; clear Hty.
+      eapply termGen' in Hty' as [? [Hty' _]].
+      inversion Hty' ; subst ; clear Hty'.
+      econstructor ; fold_decl.
+      + now econstructor.
+      + now eapply IHA.
+      + eapply IHB ; tea.
+        eapply stability ; tea.
+        econstructor.
+        1: eapply ctx_conv_refl ; gen_typing.
+        now econstructor.
+    - intros * ? ? ? IH Hf Hg.
+      assert [Γ |-[de] A].
+      {
+        eapply validity in Hf.
+        inversion Hf ; subst ; clear Hf.
+        1: eassumption.
+        eapply termGen' in H2 as [? [Hty ]].
+        inversion Hty ; subst ; clear Hty.
+        now econstructor.
+      }
+      econstructor ; tea ; fold_decl.
+      eapply IH.
+      all: now eapply typing_eta'.
+    - intros * ? IHm ? Htym Htyn.
+      edestruct IHm as [? Hm'].
+      1-2: now eexists.
+      eapply TermConv ; tea ; fold_decl.
+      now eapply Hm'.
+  Qed.
+
+End Soundness.
+
+Section Transitivity.
+
+  Let PTy (Γ : context) (A : term) := forall Γ',
+    [|-[de] Γ' ≅ Γ] -> [Γ' |-[al] A].
+  Let PInf (Γ : context) (A t : term) := forall Γ',
+    [|-[de] Γ' ≅ Γ] ->
+    ∑ A', [Γ' |-[al] t ▹ A'] × [Γ' |-[de] A' ≅ A].
+  Let PInfRed (Γ : context) (A t : term) := forall Γ',
+    [|-[de] Γ' ≅ Γ] ->
+    ∑ A', [Γ' |-[al] t ▹h A'] × [Γ' |-[de] A' ≅ A].
+  Let PCheck (Γ : context) (A t : term) := forall Γ' A',
+    [|-[de] Γ' ≅ Γ] -> [Γ' |-[de] A ≅ A'] ->
+    [Γ' |-[al] t : A'].
+  Let PTyEq (Γ : context) (A B : term) := forall Γ' A' B',
+    [|-[de] Γ' ≅ Γ] ->
+    [Γ' |-[de] A' ≅ A] ->
+    [Γ' |-[de] B ≅ B'] ->
+    [Γ' |-[al] A' ≅ B'].
+  Let PTyRedEq (Γ : context) (A B : term) := forall Γ' A' B',
+    [|-[de] Γ' ≅ Γ] ->
+    [Γ' |-[de] A' ≅ A] -> [Γ' |-[de] B ≅ B'] ->
+    [Γ' |- A' ≅h B'].
+  Let PNeEq (Γ : context) (A t u : term) := forall Γ' t' u',
+    [|-[de] Γ' ≅ Γ] ->
+    whne t' -> whne u' ->
+    [Γ' |-[de] t' ≅ t : A] -> [Γ' |-[de] u ≅ u' : A] ->
+    ∑ A', [Γ' |-[al] t' ~ u' ▹ A'] × [Γ' |-[de] A' ≅ A].
+  Let PNeRedEq (Γ : context) (A t u : term) := forall Γ' t' u',
+    [|-[de] Γ' ≅ Γ] ->
+    whne t' -> whne u' ->
+    [Γ' |-[de] t' ≅ t : A] -> [Γ' |-[de] u ≅ u' : A] ->
+    ∑ A', [Γ' |- t' ~h u' ▹ A'] × [Γ' |-[de] A' ≅ A].
+  Let PTmEq (Γ : context) (A t u : term) := forall Γ' A' t' u',
+  [|-[de] Γ' ≅ Γ] -> [Γ' |-[de] A ≅ A'] ->
+  [Γ' |-[de] t' ≅ t : A'] -> [Γ' |-[de] u ≅ u' : A'] ->
+  [Γ' |-[al] t' ≅ u' : A'].
+  Let PTmRedEq (Γ : context) (A t u : term) := forall Γ' A' t' u',
+  [|-[de] Γ' ≅ Γ] -> [Γ' |-[de] A ≅ A'] ->
+  [Γ' |-[de] t' ≅ t : A'] -> [Γ' |-[de] u ≅ u' : A'] ->
+  [Γ' |- t' ≅h u' : A'] × [Γ' |-[de] A' ≅ A].
+
+  Theorem typing_trans :
+    WfAlgoInductionConcl PTy PInf PInfRed PCheck PTyEq PTyRedEq
+      PNeEq PNeRedEq PTmEq PTmRedEq.
+  Proof.
+    apply WfAlgoInduction.
+    - econstructor.
+    - intros * ? IHA ? IHB.
+      econstructor ; unfold PTy in * ; fold_algo.
+      1: easy.
+      eapply IHB.
+      econstructor ; tea.
+      eapply TypeRefl ; fold_decl.
+  Admitted.
+
+End Transitivity.
+
+Module AlgorithmicTypingProperties.
+  Include AlgorithmicTypingData.
+
+  #[export, refine] Instance WfCtxAlgProperties : WfContextProperties (ta := al) := {}.
+  Proof.
+    all: now constructor.
+  Qed.
+
+  #[export, refine] Instance WfTypeAlgProperties : WfTypeProperties (ta := al) := {}.
+  Proof.
+    2-4: now econstructor.
+    intros.
+    now eapply typing_alg_wk.
+  Qed.
+
+  #[export, refine] Instance InferringAlgProperties : InferringProperties (ta := al) := {}.
+  Proof.
+    - intros.
+      now eapply typing_alg_wk.
+    - now econstructor.
+    - econstructor.
+      all: now eapply infer_red_equiv.
+    - now econstructor.
+    - econstructor.
+      1: now eapply infer_red_equiv.
+      eassumption. 
+  Qed.  
+
+  #[export, refine] Instance TypingAlgProperties : TypingProperties (ta := al) := {}.
+  Proof.
+    - intros.
+      now eapply typing_alg_wk.
+    - intros.
+      now econstructor.
+    - intros * Hc ?.
+      destruct Hc as [? ? ? ? ? Hc].
+      destruct Hc.
+      econstructor ; fold_algo ; tea.
+      econstructor ; fold_algo.
+      2: etransitivity.
+      all: eassumption.
+    - intros * Hc ?.
+      destruct Hc.
+      econstructor ; fold_algo ; tea.
+      red.
+      admit.
+  Admitted.
+
+  #[export, refine] Instance ConvTypeAlgProperties : ConvTypeProperties (ta := al) := {}.
+  Proof.
+  Admitted.
+
+  #[export, refine] Instance ConvTermAlgProperties : ConvTermProperties (ta := al) := {}.
+  Proof.
+  Admitted.
+
+  #[export, refine] Instance ConvNeuAlgProperties : ConvNeuProperties (ta := al) := {}.
+  Proof.
+  Admitted.
+
+  Lemma RedTermAlgProperties :
+    RedTermProperties (ta := al).
+  Proof.
+  Admitted.
+
+  #[export]Existing Instance RedTermAlgProperties.
+
+  Lemma RedTypeAlgProperties :
+    RedTypeProperties (ta := al).
+  Proof.
+  Admitted.
+
+  #[export] Existing Instance RedTypeAlgProperties.
+
+  #[export] Instance AlgorithmicTypingProperties : GenericTypingProperties al _ _ _ _ _ _ _ _ _ := {}.
+
+End AlgorithmicTypingProperties.
